theories/Compiler/pipeline_correctness.v
@@ -1,0 +1,76 @@
+Definition opts := default_opts.
+
+Definition run_pipeline p pre :=
+  let p' := Transform.Transform.run (certirocq_post_metarocq_pipeline econf) p pre in
+  let (perr, log) := run_pipeline _ _ opts p' (compile_LambdaANF_ANF next_id []) in
+  match perr with
+  | Ret p =>
+    let '(pr, cenv, _, _, nenv, fenv, idm,  e) := p in
+    Some (nenv, cenv, idm, e)
+  | Err s => None
+  end.
+
+  Let Hf_src := LambdaBox_resource_fuel.
+  Let Ht_src := LambdaBox_resource_trace.
+  
+  Existing Instance default_wcbv_flags.
+
+
+
+
+  Context {fuel trace : Type}.
+  Context {Hf : @fuel_resource fuel} {Ht : @trace_resource trace}.
+(* Transparent bind. *)
+(* Transparent Pipeline_utils.ret. *)
+
+
+  Theorem correctness_from_erasure' (p : EProgram.eprogram) : 
+
+  forall pre : Transform.Transform.pre (verified_lambdabox_pipeline econf) p,
+  forall v, 
+    EWcbvEval.eval (fst p) (snd p) v ->
+    exists nenv cenv cm e ev v' n r fuel trace, 
+      run_pipeline p pre = Some (nenv, cenv, e) /\
+      @eval_env_step _ Hf_src Ht_src [] [] v (Val v') n r /\
+      eval.bstep_fuel (Hf:=Hf) (Ht := Ht) (snd nenv) emp e fuel (eval.Res ev) trace /\
+      anf_util.anf_val_rel (Hf_src := Hf_src) (Ht_src:=Ht_src) func_tag default_tag tgm cm (fst p) v' ev.
+  Proof.
+    intros pre v ev.
+    unfold run_pipeline.
+    unfold Pipeline_utils.run_pipeline, runState.
+    unfold Transform.Transform.run, Transform.time.
+    set (tr := Transform.Transform.transform _ _ _).
+    unfold compile_LambdaANF_ANF. unfold debug_msg, get_options, compM.ask. unfold opts, default_opts.
+    cbn -[tr].
+    destruct (LambdaANF_ANF _ _ _ ) eqn:ela.
+    unfold LambdaANF_ANF in ela.
+    Search anf.convert_top_anf. 
+
+
+    { exfalso.
+      unfold LambdaANF
+    
+    }
+    cbn. destruct get_options. cbn. 
+    Set Printing All. unfold tmBind. cbn.
+
+
+
+
+
+
+From MetaRocq.Template Require Import WcbvEval TemplateProgram.
+
+Theorem correctness mapping (p : template_program) : 
+  Transform.Transform.pre (erasure_pipeline_mapping econf) (mapping, p) ->
+  forall v, 
+    eval (fst p) (snd p) v ->
+    exists nenv cenv fuel trace e v' n r, 
+      run_pipeline p = Some (nenv, cenv, e) /\ 
+      eval.bstep_fuel cenv emp e fuel (eval.Res v1) trace /\
+      eval_env_step [] v v' n r.
+
+
+
+
+*)
